theories/simplang/examples/reorder_malloc.v
@@ -41,7 +41,8 @@ Section reorder.
     iApply (sim_bij_insert with "Ha1_t Ha2_s Hl1_t Hl2_s Hv1"); iIntros "#Hbij_1".
     iApply (sim_bij_insert with "Ha2_t Ha1_s Hl2_t Hl1_s Hv2"); iIntros "#Hbij_2".
 
-    iApply sim_call; [done | done | simpl; by eauto ].
+    iApply sim_wand; [ iApply sim_call; [done | done | simpl; by eauto ] |].
+    iIntros (??) "$".
   Qed.
 
 End reorder.
