theories/simplang/proofmode.v
@@ -12,7 +12,7 @@ From iris.prelude Require Import options.
 
 Section sim.
 Context `{!sheapGS Σ} `{sheapInv Σ}.
-Context (Ω : val → val → iProp Σ) (π : thread_id).
+Context (Ω : thread_id → val → val → iProp Σ) (π : thread_id).
 Local Notation "et '⪯' es {{ Φ }}" := (et ⪯{π, Ω} es {{Φ}})%I (at level 40, Φ at level 200) : bi_scope.
 Local Notation "et '⪯' es [{ Φ }]" := (et ⪯{π, Ω} es [{Φ}])%I (at level 40, Φ at level 200) : bi_scope.
 
